prophecy counterexample

theories/examples/counterexample.v
@@ -4,7 +4,7 @@ Set Default Proof Using "Type*".
 (** If we assume that we can freely pick presampling tapes to read from when
     resolving probabilistic choices, we can show refinements/equivalences that
     do not hold. *)
-Section counterexample.
+Section counterexample_annotation.
   Context `{!clutchRGS Σ}.
 
   (** An (unsound) rule that allows us to pick an arbitrary presampling tape
@@ -23,7 +23,7 @@ Section counterexample.
 
   (** If we assume [refines_tape_unsound], we can show that [flip] refines
       [flip_ors] which obviously cannot true. *)
-  Lemma counterexample α1 α2 :
+  Lemma counterexample_annotation α1 α2 :
     refines_tape_unsound →
     α1 ↪B [] ∗ α2 ↪B []
     ⊢ REL flip << flip_ors  : lrel_bool.
@@ -42,4 +42,99 @@ Section counterexample.
       iFrame. iIntros "Hα2". rel_values.
   Qed.
 
-End counterexample.
+End counterexample_annotation.
+
+(** This counter example shows that prophecy variables (as developed for
+    HeapLang in Iris) is unsound for the coupling logic, for the same reason
+    that presampling is unsound without syntatic tape labels: If you can predict
+    the outcomes of random samples ahead of time, it gives you too much power to
+    choose which sampling you couple with. *)
+Section counterexample_prophecies.
+  Context `{!clutchRGS Σ}.
+
+  (** We assume prophecy variables exist in our language with [WP] specs as
+      found in [HeapLang] (see https://dl.acm.org/doi/10.1145/3371113) *)
+  Class prophecies := {
+      NewProph : val;
+      ResolveProph : val;
+      proph_id : Set;
+      proph : proph_id → list (val * val) → iProp Σ;
+      LitProphecy : proph_id → base_lit;
+
+      wp_new_proph s E :
+        {{{ True }}}
+          NewProph #() @ s; E
+        {{{ pvs p, RET (LitV (LitProphecy p)); proph p pvs }}};
+
+     wp_resolve_proph s E (p : proph_id) (pvs : list (val * val)) v :
+       {{{ proph p pvs }}}
+         ResolveProph (Val $ LitV $ LitProphecy p) (Val v) @ s; E
+       {{{ pvs', RET (LitV LitUnit); ⌜pvs = (LitV LitUnit, v)::pvs'⌝ ∗ proph p pvs' }}};
+    }.
+
+  (** [flip_ands] return true with probability 1/4, false with 3/4  *)
+  Definition flip_ands `{prophecies} : expr :=
+    let: "p" := NewProph #() in
+    let: "x" := flip in
+    let: "y" := flip in
+    ResolveProph "p" "y";;
+    "x" && "y".
+
+  (** We show that [flip_ands] refines [flip] which can cannot be true. *)
+  Lemma counterexample_prophecies `{prophecies} :
+    ⊢ REL flip_ands << flip : lrel_bool.
+  Proof.
+    (** As we're assuming regular [WP] specs for the prophecy variables, we'll
+        unfold the relational logic and work directly in the unary logic. *)
+    rewrite refines_eq /refines_def /=.
+    iIntros (K) "Hr Hna". rewrite /flip_ands.
+    wp_apply wp_new_proph; [done|].
+    iIntros (pvs p) "Hp".
+    wp_pures.
+    destruct pvs as [|(?&v) ?].
+    { (** Contradictory case -- we will resolve the prophecy in the program so
+          the list of prophecies is non-empty *)
+      wp_apply wp_flip; [done|]; iIntros (b1) "_". wp_pures.
+      wp_apply wp_flip; [done|]; iIntros (b2) "_". wp_pures.
+      wp_apply (wp_resolve_proph with "Hp").
+      iIntros (?) "(% & ?)". simplify_eq. }
+    (** Prophecies resolve a priori to any value in the language, but we will
+        only resolve it to a Bool in the program *)
+    assert ((∃ b : bool, v = #b) ∨ ∀ b : bool, v ≠ #b) as Hcases.
+    { destruct v; firstorder. destruct l; firstorder. eauto. }
+    destruct Hcases as [Hbool|]; last first.
+    { (** Contradictory case -- we *do* resolve the prophecy to a Bool *)
+      wp_apply wp_flip; [done|]; iIntros (b1) "_". wp_pures.
+      wp_apply wp_flip; [done|]; iIntros (b2) "_". wp_pures.
+      wp_apply (wp_resolve_proph with "Hp").
+      iIntros (?) "(% & ?)". congruence. }
+
+    (** Now, we're in the interesting situation. We case on the Boolean content
+        of the prophecy. *)
+    destruct Hbool as [[] ->].
+    - (** The prophecy was [true], and we do an identity coupling with the
+          [flip] of [x]. This guarantees that the result of [x && true] on the
+          left agrees with the result of the [flip] on the right. *)
+      wp_apply wp_couple_flip_flip; [done|].
+      iFrame "Hr". iIntros "/= !>" (b) "Hr".
+      wp_pures.
+      wp_apply wp_flip; [done|]; iIntros (b2) "_". wp_pures.
+      wp_apply (wp_resolve_proph with "Hp").
+      iIntros (?) "[% Hp]". simplify_eq.
+      destruct b; wp_pures;
+        iModIntro; iExists _; eauto with iFrame.
+    - (** The prophecy is [false], and we do an identity coupling with the
+          [flip] of [y]. The result of the left is predetermined to be [x &&
+          false = false]. By coupling [y] (that we know will be [false]) with
+          the [flip] on the right, we guarantee that the right also evaluates to
+          [false]. *)
+      wp_apply wp_flip; [done|]; iIntros (b1) "_". wp_pures.
+      wp_apply wp_couple_flip_flip; [done|]. iFrame.
+      iIntros "/= !>" (b2) "Hr". wp_pures.
+      wp_apply (wp_resolve_proph with "Hp").
+      iIntros (?) "[% Hp]". simplify_eq. wp_pures.
+      destruct b1; wp_pures;
+        iModIntro; iExists _; eauto with iFrame.
+  Qed.
+
+End counterexample_prophecies.
